Copied checks-effects-interactions-pattern approach This is as it was for the FMBC paper. An important issue it has is that it allows balance checks after an "interaction", this needs to be fixed (and will be) as it is unsafe with regards to the checks-effects-interactions pattern.

Edsger/coqgen.ml
@@ -2589,6 +2589,27 @@ Section OBJECT_" ^ i ^ "_DEFINITION.
     @apply_param_func " ^ method_full_name ^ ".(FC_params) _
                       (" ^ method_full_name ^ "_opt) args.
 
+(* CEI stands for Checks Effects Interactions (pattern) and the definitions below are used
+    to keep track of the safe situations in which a primitive can be called. See also
+    cmd_constr_CEI_pattern_prf in Syntax.v and for the tactic definitions see Runtime.v *)
+    
+Lemma " ^ method_full_name ^ "_CEI_AB : { rsts | function_constr_CEI_pattern_prf (fst rsts) " ^ method_full_name ^ " (snd rsts)}.
+Proof.
+  unfold " ^ method_full_name ^ ".
+  CEI_auto_AB. (* If this tactic fails then it indicates that a strict version of the Checks-Effects-Interactions pattern was not followed in the function: " ^ method_full_name ^ ". *)
+Defined.
+
+Lemma " ^ method_full_name ^ "_CEI_BA : { rsts | function_constr_CEI_pattern_prf (fst rsts) " ^ method_full_name ^ " (snd rsts)}.
+Proof.
+  unfold " ^ method_full_name ^ ".
+  CEI_auto_BA.
+Defined.
+
+Definition " ^ method_full_name ^ "_CEI_rsts_before_A := fst (proj1_sig " ^ method_full_name ^ "_CEI_AB).
+Definition " ^ method_full_name ^ "_CEI_rsts_after_A := snd (proj1_sig " ^ method_full_name ^ "_CEI_AB).
+Definition " ^ method_full_name ^ "_CEI_rsts_before_B := fst (proj1_sig " ^ method_full_name ^ "_CEI_BA).
+Definition " ^ method_full_name ^ "_CEI_rsts_after_B := snd (proj1_sig " ^ method_full_name ^ "_CEI_BA).
+
   Definition " ^ method_full_name ^ "_prim := {|
     PRIMident := ident_" ^ o.aObjectName ^ "_" ^ m.aMethodName ^ ";
     (* PRIMcc := AST.cc_default; *)
@@ -2597,6 +2618,10 @@ Section OBJECT_" ^ i ^ "_DEFINITION.
     PRIMpure := " ^ string_of_bool is_pure ^ ";
     PRIMargt_marker := " ^ method_full_name ^ ".(FC_params);
     PRIMret_marker := " ^ method_full_name ^ ".(FC_returns);
+    PRIMrst_before_A := " ^ method_full_name ^ "_CEI_rsts_before_A;
+    PRIMrst_after_A := " ^ method_full_name ^ "_CEI_rsts_after_A;
+    PRIMrst_before_B := " ^ method_full_name ^ "_CEI_rsts_before_B;
+    PRIMrst_after_B := " ^ method_full_name ^ "_CEI_rsts_after_B;
     PRIMcond := fun _ _ _ => True;
     (* PRIMsem := " ^ method_full_name ^ "_spec_hlist; *)
     PRIMsem_opt := " ^ method_full_name ^ "_spec_hlist_opt
