core/Syntax.v
@@ -180,7 +180,18 @@ Section STMT_CONSTR.
   apply Monad_option.
   apply Zero_option.
   Defined.
-  
+
+
+Inductive checks_effects_interactions_pattern_state :=
+  | Safe_no_reentrancy
+  | Safe_with_potential_reentrancy.
+
+  (*  The underlay interface for a primitive is a Coq Prop, a relation from memory etc to the final value.
+      But we want a Coq function. So the primitive record contains the function.
+
+      Then the class primitive_exec_prf says that the primitive is equivalent to the specification in the
+      underlay interface.
+   *)
   Record primitive (argt : list hyper_type_pair)(ret : hyper_type_pair)
       : Type := mk_prim {
     PRIMident : ident;
@@ -190,7 +201,34 @@ Section STMT_CONSTR.
     PRIMpure  : bool;                 
     PRIMargt_marker : type_marker argt;
     PRIMret_marker : type_marker ret;
-    
+    (* PRIMrst_before/after_A/B relate to reentrancy tracking using the Checks Effects 
+    Interactions pattern. They represent the safe state(s) the prim can be executed
+    in and the resulting checks_effects_interactions_pattern_state afterwards.
+    In particular they should be one of the following:
+      
+      When a prim has only safe commands:
+      Safe_no_reentrancy, Safe_no_reentrancy
+      Safe_with_potential_reentrancy, Safe_with_potential_reentrancy
+      
+      When a prim has commands only safe before reentrancy:
+      Safe_no_reentrancy, Safe_no_reentrancy
+      Safe_no_reentrancy, Safe_no_reentrancy (repeated)
+      
+
+      When a prim has a command that introduces reentrancy:
+      Safe_no_reentrancy, Safe_with_potential_reentrancy
+      Safe_no_reentrancy, Safe_with_potential_reentrancy (repeated)
+
+    The relevant values are filled in automatically.
+      *)
+      PRIMrst_before_A : checks_effects_interactions_pattern_state;
+      PRIMrst_after_A : checks_effects_interactions_pattern_state;
+      PRIMrst_before_B : checks_effects_interactions_pattern_state;
+      PRIMrst_after_B : checks_effects_interactions_pattern_state;
+
+    (* PRIMsem_opt, the "monadic" version, combines PRIMcond and PRIMsem into one thing.
+       There is a verification condition below saying that they must be equivalent;
+       the synthesis use them interchangably for convenience. *)
     PRIMcond : HList tp_ft argt -> machine_env GetHighData -> GetHighData -> Prop;
     PRIMsem_opt : HList tp_ft argt -> machine_env GetHighData -> DS (tp_ft ret)
   }.
@@ -497,3 +535,158 @@ Section CONSTR_PRF.
   
   
 End CONSTR_PRF.
+
+Section CEIP_PRF.
+  Context `{HM : HyperMem}.
+
+
+Inductive cmd_constr_CEI_pattern_prf :
+
+(*  Abbreviations:
+      CEI = Checks-Effects-Interactions (pattern)
+      cmd = command
+      prf = proof
+      CCCEIP___ = Command Constructor Check Effects Interactions (pattern) Proof ___
+      r = return type (of the command)
+      r1 = return type 1
+      c1 = command 1
+      rst = reentrancy safety state
+      e = expression
+  *)
+
+  forall ret,
+    checks_effects_interactions_pattern_state -> cmd_constr ret -> checks_effects_interactions_pattern_state -> Prop :=
+    (* In the type of cmd_constr_CEI_pattern_prf, the first occurance of checks_effects_interactions_pattern_state corresponds to the checks_effects_interactions_pattern_state before executing the command, and the last checks_effects_interactions_pattern_state corresponds to the checks_effects_interactions_pattern_state after executing the command. *)
+| CCCEIPskip :
+    forall {rst},
+      cmd_constr_CEI_pattern_prf _ rst CCskip rst
+      (* "skip" leaves rst unchaged *)
+| CCCEIPlet :
+    forall {rst1} {rst2} {rst3} r `{ht : HyperType tp} id c1 c2,
+      cmd_constr_CEI_pattern_prf (mk_hyper_type_pair tp) rst1 c1 rst2 ->
+      cmd_constr_CEI_pattern_prf r rst2 c2 rst3 ->
+      cmd_constr_CEI_pattern_prf r rst1 (CClet id c1 c2) rst3
+      (* "let" leaves rst as the rst from running c1 then c2 *)
+| CCCEIPload : 
+    forall `{ht : HyperType tp} e,
+      cmd_constr_CEI_pattern_prf _ Safe_no_reentrancy (CCload e) Safe_no_reentrancy
+      (* "load" can only be run safely from Safe_no_reentrancy, and leaves it rst as Safe_no_reentrancy *)
+| CCCEIPstore :
+    forall `{ht : HyperType tp} el er,
+      cmd_constr_CEI_pattern_prf _ Safe_no_reentrancy (CCstore el er) Safe_no_reentrancy
+      (* "store" can only be run safely from Safe_no_reentrancy, and leaves it rst as Safe_no_reentrancy *)
+| CCCEIPsequence :
+    forall {rst1} {rst2} {rst3} r (c1 : cmd_constr void_unit_pair) (c2 : cmd_constr r),
+      cmd_constr_CEI_pattern_prf void_unit_pair rst1 c1 rst2 ->
+      cmd_constr_CEI_pattern_prf r rst2 c2 rst3 ->
+      cmd_constr_CEI_pattern_prf r rst1 (CCsequence c1 c2) rst3
+      (* "sequence" leaves rst as the rst from running c1 then c2 *)      
+
+(* "ifthenelse" is split into the five allowable cases (rather than using a match statement) to simplify the type-checking. *)
+(* Here we assume the worst case scenario, I guess it would be nice to be able to analyse the truth value of e here. *)
+(* "ifthenelse" leaves rst as the rst from assuming the worst case scenario out of the commands in the branches *)
+| CCCEIPifthenelse1 : (* Safe_no_reentrancy Safe_no_reentrancy Safe_no_reentrancy *)
+  forall r e c_true c_false,
+    cmd_constr_CEI_pattern_prf r Safe_no_reentrancy c_true Safe_no_reentrancy ->
+    cmd_constr_CEI_pattern_prf r Safe_no_reentrancy c_false Safe_no_reentrancy ->
+    cmd_constr_CEI_pattern_prf r Safe_no_reentrancy (CCifthenelse e c_true c_false) Safe_no_reentrancy      
+| CCCEIPifthenelse2 : (* Safe_no_reentrancy Safe_with_potential_reentrancy Safe_no_reentrancy *)
+  forall r e c_true c_false,
+    cmd_constr_CEI_pattern_prf r Safe_no_reentrancy c_true Safe_with_potential_reentrancy ->
+    cmd_constr_CEI_pattern_prf r Safe_no_reentrancy c_false Safe_no_reentrancy ->
+    cmd_constr_CEI_pattern_prf r Safe_no_reentrancy (CCifthenelse e c_true c_false) Safe_with_potential_reentrancy      
+| CCCEIPifthenelse3 : (* Safe_no_reentrancy Safe_no_reentrancy Safe_with_potential_reentrancy *)
+  forall r e c_true c_false,
+    cmd_constr_CEI_pattern_prf r Safe_no_reentrancy c_true Safe_no_reentrancy ->
+    cmd_constr_CEI_pattern_prf r Safe_no_reentrancy c_false Safe_with_potential_reentrancy ->
+    cmd_constr_CEI_pattern_prf r Safe_no_reentrancy (CCifthenelse e c_true c_false) Safe_with_potential_reentrancy      
+| CCCEIPifthenelse4 : (* Safe_no_reentrancy Safe_with_potential_reentrancy Safe_with_potential_reentrancy *)
+  forall r e c_true c_false,
+    cmd_constr_CEI_pattern_prf r Safe_no_reentrancy c_true Safe_with_potential_reentrancy ->
+    cmd_constr_CEI_pattern_prf r Safe_no_reentrancy c_false Safe_with_potential_reentrancy ->
+    cmd_constr_CEI_pattern_prf r Safe_no_reentrancy (CCifthenelse e c_true c_false) Safe_with_potential_reentrancy      
+| CCCEIPifthenelse5 : (* Safe_with_potential_reentrancy Safe_with_potential_reentrancy Safe_with_potential_reentrancy *)
+  forall r e c_true c_false,
+    cmd_constr_CEI_pattern_prf r Safe_with_potential_reentrancy c_true Safe_with_potential_reentrancy ->
+    cmd_constr_CEI_pattern_prf r Safe_with_potential_reentrancy c_false Safe_with_potential_reentrancy ->
+    cmd_constr_CEI_pattern_prf r Safe_with_potential_reentrancy (CCifthenelse e c_true c_false) Safe_with_potential_reentrancy      
+
+| CCCEIPfor :
+    forall {rst} id_it id_end e1 e2 c,
+      cmd_constr_CEI_pattern_prf _ rst c rst ->
+      cmd_constr_CEI_pattern_prf _ rst (CCfor id_it id_end e1 e2 c) rst
+      (* This is slightly overly restrictive, for example a for loop that actually only loops once and contains a transferEth call will not be allowed. *)
+    (* "for" probably loops through c many times, so to be safe we assume it can only be run safely if c is a command which results in rst (and starts from rst). Then the loop as a whole is only safe if started from rst and will result in a rst state. *)
+| CCCEIPfirst :
+    forall {rst} r id_it id_end id_dest e1 e2 c3 c4 c5,
+      cmd_constr_CEI_pattern_prf int_bool_pair rst c3 rst ->
+      cmd_constr_CEI_pattern_prf r rst c4 rst ->
+      cmd_constr_CEI_pattern_prf r rst c5 rst ->
+      cmd_constr_CEI_pattern_prf r rst
+                    (CCfirst id_it id_end id_dest e1 e2 c3 c4 c5)
+                    rst
+            (* Slightly over-restrictive, like for. Also the command that executes when the loop exits could move rst from Safe_no_reentrancy to Safe_with_potential_reentrancy, but this, being overly restrictive would not allow that (fairly unlikely) situation. *)
+      (* With "first", similarly to "for" we assume all the commands (which may be looped) result in rst (and start from rst). So the overall first-loop is only safe if started from rst and will result in a rst state. *)
+| CCCEIPfold :
+    forall `{ht : HyperType tp} {rst} id_it id_end id_recur id_dest e1 e2 e3 c,
+      cmd_constr_CEI_pattern_prf _ rst c rst ->
+      cmd_constr_CEI_pattern_prf _
+        rst
+        (CCfold id_it id_end id_recur id_dest e1 e2 e3 c)
+        rst
+        (* Similarly to CCCEIPfor, this is overly restrictive. *)
+    (* With "fold", similarly to "for" and "first" we assume all the commands (which may be looped) result in rst (and start from rst). So the overall fold is only safe if started from rst and will result in a rst state. *)
+| CCCEIPcall1 :
+    forall {rst1} {rst2} r argt prim arg,
+      rst1 = prim.(PRIMrst_before_A argt r) -> rst2 = prim.(PRIMrst_after_A argt r) -> cmd_constr_CEI_pattern_prf r rst1 (CCcall prim arg) rst2
+| CCCEIPcall2 :
+    forall {rst1} {rst2} r argt prim arg (IHprim : @primitive_prf _ _ argt r prim),
+      rst1 = prim.(PRIMrst_before_B argt r)-> rst2 = prim.(PRIMrst_after_B argt r) -> cmd_constr_CEI_pattern_prf r rst1 (CCcall prim arg) rst2
+    (* "call" should result in the same rst as the primitive being called, and be safe to call in the same circumstances as the primitive is called.
+        The primitives will have automatically generated fields rst_before/after_A/B to describe the safe ways in which prim can be called. *)
+(* | CCCEIPcall_ext : 
+        (* Note: this should be similar to CCCEIPtransfer and also to CCPcall_ext *)
+*)
+| CCCEIPyield :
+    forall {rst} `{ht : HyperType tp} e,
+      cmd_constr_CEI_pattern_prf _ rst (CCyield e) rst
+    (* "yield" retains the current rst *)
+| CCCEIPconstr :
+    forall `{ht : HyperType tp} fld_ids fld_tps el flds constr,
+      cmd_constr_CEI_pattern_prf _ Safe_no_reentrancy (CCconstr fld_ids fld_tps el flds constr) Safe_no_reentrancy
+      (* "constr" assigns to storage so can only be called if Safe_no_reentrancy, and does not introduce the possiblity of reentrancy itself. *)
+| CCCEIPtransfer :
+    forall e1 e2,
+      cmd_constr_CEI_pattern_prf _ Safe_no_reentrancy (CCtransfer e1 e2) Safe_with_potential_reentrancy
+      (* What this is all about, "transfer" can only be called in a Safe_no_reentrancy state and DOES introduce potential reentrancy. *)
+| CCCEIPassert :
+    forall {rst1} {rst2} c,
+      cmd_constr_CEI_pattern_prf _ rst1 c rst2 -> cmd_constr_CEI_pattern_prf _ rst1 (CCassert c) rst2
+    (* "assert" results in the same rst (and can be called safely in the same situations as) the command c *)
+| CCCEIPdeny :
+    forall {rst1} {rst2} c,
+      cmd_constr_CEI_pattern_prf _ rst1 c rst2 -> cmd_constr_CEI_pattern_prf _ rst1 (CCdeny c) rst2
+  (* "deny" results in the same rst (and can be called safely in the same situations as) the command c *)
+| CCCEIPpanic :
+    forall {rst} `{ht : HyperType},
+      cmd_constr_CEI_pattern_prf _ rst (CCpanic tp) rst
+  (* "panic" retains the current rst *)
+| CCCEIPrespec :
+    forall {rst1} {rst2} r tmp' c spec,
+      cmd_constr_CEI_pattern_prf r rst1 c rst2 -> 
+      cmd_constr_CEI_pattern_prf r rst1 (CCrespec tmp' c spec) rst2
+  (* "respec" results in the same rst (and can be called safely in the same situations as) the command c *)
+| CCCEIPrespec_opt : 
+    forall {rst1} {rst2} r tmp' c spec,
+      cmd_constr_CEI_pattern_prf r rst1 c rst2 -> 
+      cmd_constr_CEI_pattern_prf r rst1 (CCrespec_opt tmp' c spec) rst2
+  (* "respec_opt" results in the same rst (and can be called safely in the same situations as) the command c *)
+.
+
+Definition function_constr_CEI_pattern_prf 
+    (rst_before : checks_effects_interactions_pattern_state)
+    (f : function_constr)
+    (rst_after : checks_effects_interactions_pattern_state) :=
+       cmd_constr_CEI_pattern_prf f.(FC_returns) rst_before f.(FC_body) rst_after.
+
+End CEIP_PRF.
