Runtime.v
@@ -858,3 +858,63 @@ Proof.
   apply Zmod_small.
   apply Int.Z_mod_modulus_range.
 Qed.
+
+(* Tactics related to reentrancy tracking using the Checks Effects Interactions Pattern: *)
+
+(* CEI_auto tries to solve a goal of the form 
+   cmd_constr_CEI_pattern_prf ____ rst_before _____ rst_after
+*)
+Ltac CEI_auto :=
+  repeat (
+  reflexivity
++ typeclasses eauto 
++ eapply CCCEIPskip
++ eapply CCCEIPlet 
++ eapply CCCEIPload  
++ eapply CCCEIPstore 
++ eapply CCCEIPsequence 
++ eapply CCCEIPifthenelse1 
++ eapply CCCEIPifthenelse2 
++ eapply CCCEIPifthenelse3 
++ eapply CCCEIPifthenelse4 
++ eapply CCCEIPifthenelse5 
++ eapply CCCEIPfor 
++ eapply CCCEIPfirst 
++ eapply CCCEIPfold 
++ eapply CCCEIPcall1 
++ eapply CCCEIPcall2 
++ eapply CCCEIPyield 
++ eapply CCCEIPconstr 
++ eapply CCCEIPtransfer 
++ eapply CCCEIPassert 
++ eapply CCCEIPdeny 
++ eapply CCCEIPpanic 
++ eapply CCCEIPrespec 
++ eapply CCCEIPrespec_opt)
+  .
+
+(* CEI_auto_states_A tries to solve a CEI goal by trying the pairs of states shown below. *)
+Ltac CEI_auto_states_A := 
+  solve [
+      (simpl; exists (Safe_no_reentrancy, Safe_no_reentrancy); CEI_auto)
+    | (simpl; exists (Safe_no_reentrancy, Safe_with_potential_reentrancy); CEI_auto)
+  ].
+
+(* CEI_auto_states_B tries to solve a CEI goal by trying the pairs of states shown below. *)
+Ltac CEI_auto_states_B := 
+  solve [
+      (simpl; exists (Safe_with_potential_reentrancy, Safe_with_potential_reentrancy); CEI_auto)
+  ].
+
+(* CEI_auto_AB tries to solve a CEI goal by first trying the pairs of states from CEI_auto_states_A
+     then CEI_auto_states_B. *)
+Ltac CEI_auto_AB :=
+  solve [CEI_auto_states_A | CEI_auto_states_B].
+
+(* CEI_auto_BA tries to solve a CEI goal by first trying the pairs of states from CEI_auto_states_B
+     then CEI_auto_states_A. *)
+Ltac CEI_auto_BA :=
+  solve [CEI_auto_states_B | CEI_auto_states_A].
+
+(* CEI_auto_AB and BA are intended to be used to generate the PRIMrst_before/after_A/B entries in 
+  _prim entries, later used in higher level cmd_constr_CEI_pattern_prf goals. *)
